$\langle \mathbf{0}, \mathbf{v} \rangle = \langle \mathbf{v}, \mathbf{0} \rangle = 0$.

## Proof

\[ \langle \mathbf{0}, \mathbf{v} \rangle
= \langle \mathbf{0} + \mathbf{0}, \mathbf{v} \rangle
= \langle \mathbf{0}, \mathbf{v} \rangle + \langle \mathbf{0}, \mathbf{v} \rangle \tag{linearity in first argument}
\Rightarrow \langle \mathbf{0}, \mathbf{v} \rangle = 0 \]

\[ \langle \mathbf{v}, \mathbf{0} \rangle
= \overline{\langle \mathbf{0}, \mathbf{v} \rangle} \tag{conjugate symmetry}
= \overline{0} = 0 \]
