Let $N$ be a normal subgroup of $G$. This means that $gN = Ng$ for all $g \in G$.
The coset of a normal subgroup is called a normal coset.

Define the product of cosets $aN$ and $bN$ as
\[ (aN)(bN) = (ab)N \]

This product is well-defined, which means that it does not depend on the representation of the coset.
This means that
\[ a_1N = a_2N \wedge b_1N = b_2N \Rightarrow (a_1N)(b_1N) = (a_2N)(b_2N) \]

## Proof

\begin{align}
& (a_1N)(b_1N) &= (a_1b_1)N
\\ &= a_1(b_1N) &= a_1(b_2N)
\\ &= a_1(Nb_2) &= (a_1N)b_2
\\ &= (a_2N)b_2 &= a_2(Nb_2)
\\ &= a_2(b_2N) &= (a_2b_2)N
\\ &= (a_2N)(b_2N)
\end{align}
